untidy but working execute_LOAD simplification

OpenvmFv/Spec/Load/local.lean
@@ -89,6 +89,76 @@ namespace Local
     vmem_read = LeanRV32D.Functions.vmem_read
   := rfl
 
+  noncomputable def vmem_read'
+    (rs : regidx) (offset : BitVec 32) (width : ℕ) (acc : AccessType Unit)
+    (aq rl res : Bool)
+  : SailM (Sail.Result (BitVec (8 * width)) ExecutionResult) := Sail.SailME.run do
+    let vaddr ← (( do
+      match (← (LeanRV32D.Functions.ext_data_get_addr rs offset acc width)) with
+      | .Ext_DataAddr_OK vaddr => (pure vaddr)
+      | .Ext_DataAddr_Error e =>
+        Sail.SailME.throw ((Sail.Err (ExecutionResult.Ext_DataAddr_Check_Failure e)) : (Sail.Result (BitVec (8 * width)) ExecutionResult))
+      ) : Sail.SailME (Sail.Result (BitVec (8 * width)) ExecutionResult) virtaddr )
+    if (res : Bool)
+    then
+      (do
+        if ((LeanRV32D.Functions.not (LeanRV32D.Functions.is_aligned_vaddr vaddr width)) : Bool)
+        then
+          Sail.SailME.throw ((Sail.Err (ExecutionResult.Memory_Exception (vaddr, (ExceptionType.E_Load_Addr_Align ())))) : (Sail.Result (BitVec (8 * width)) ExecutionResult))
+        else (pure ()))
+    else
+      (do
+        if ((LeanRV32D.Functions.check_misaligned vaddr width) : Bool)
+        then
+          Sail.SailME.throw ((Sail.Err (ExecutionResult.Memory_Exception (vaddr, (ExceptionType.E_Load_Addr_Align ())))) : (Sail.Result (BitVec (8 * width)) ExecutionResult))
+        else (pure ()))
+    let (n, bytes) ← do (LeanRV32D.Functions.split_misaligned vaddr width)
+    let data := (LeanRV32D.Functions.zeros (n := ((8 *i n) *i bytes)))
+    let (first, last, step) := (LeanRV32D.Functions.misaligned_order n)
+    let i : Nat := first
+    let finished : Bool := false
+    let vaddr := (LeanRV32D.Functions.bits_of_virtaddr vaddr)
+    let (data, _finished, _i) ← (( do
+      let loop_vars ← untilFuelM (fuel :=n) (λ (data, finished, i) => (pure finished)) (data, finished, i)
+        fun (data, finished, i) => do
+          let offset := i
+          let vaddr := (Sail.BitVec.addInt vaddr (offset *i bytes))
+          let data ← (( do
+            match (← (LeanRV32D.Functions.translateAddr (virtaddr.Virtaddr vaddr) acc)) with
+            | .Err (e, _) =>
+              Sail.SailME.throw ((Sail.Err (ExecutionResult.Memory_Exception ((virtaddr.Virtaddr vaddr), e))) : (Sail.Result (BitVec (8 * width)) ExecutionResult))
+            | .Ok (paddr, _) =>
+              (do
+                match (← (LeanRV32D.Functions.mem_read acc paddr bytes aq rl res)) with
+                | .Err e =>
+                  Sail.SailME.throw ((Sail.Err (ExecutionResult.Memory_Exception ((virtaddr.Virtaddr vaddr), e))) : (Sail.Result (BitVec (8 * width)) ExecutionResult))
+                | .Ok v =>
+                  (do
+                    if (res : Bool)
+                    then (load_reservation (LeanRV32D.Functions.bits_of_physaddr paddr))
+                    else (pure ())
+                    (pure (Sail.BitVec.updateSubrange data (((8 *i (offset +i 1)) *i bytes) -i 1)
+                        ((8 *i offset) *i bytes) v)))) ) : Sail.SailME
+            (Sail.Result (BitVec (8 * width)) ExecutionResult) (BitVec (8 * n * bytes)) )
+          let (finished, i) : (Bool × Nat) :=
+            if ((offset == last) : Bool)
+            then
+              (let finished : Bool := true
+              (finished, i))
+            else
+              (let i : Nat := (offset +i step)
+              (finished, i))
+          (pure (data, finished, i))
+      (pure loop_vars) ) : Sail.SailME (Sail.Result (BitVec (8 * width)) ExecutionResult)
+      ((BitVec (8 * n * bytes)) × Bool × Nat) )
+    (pure (Sail.Ok data))
+
+  lemma vmem_read'_equiv:
+    vmem_read =
+    vmem_read'
+  := by
+    sorry
+
   lemma ext_data_get_addr :
     LeanRV32D.Functions.ext_data_get_addr rd offset acc width =
     λ state => match LeanRV32D.Functions.rX_bits rd state with
@@ -305,6 +375,10 @@ namespace Local
         | _ => panic! "unexpected_privilege"
 
   lemma effective_privilege
+    (accessType: AccessType Unit)
+    (privilege)
+    (state)
+    (status)
     (h_status:
       Sail.BitVec.extractLsb status 12 11 = 0#2 ∨
       Sail.BitVec.extractLsb status 12 11 = 1#2 ∨
@@ -371,11 +445,10 @@ namespace Local
       Sail.BitVec.extractLsb status 12 11 = 1#2 ∨
       Sail.BitVec.extractLsb status 12 11 = 3#2
     )
-    (h_access_type: accessType != AccessType.InstructionFetch ())
     (h_satp: Sail.readReg Register.satp state = EStateM.Result.ok satp state)
     (h_translation_mode: translation_mode_pure satp (effective_privilege_pure status privilege) == SATPMode.Bare)
   :
-    LeanRV32D.Functions.translateAddr addr accessType state =
+    LeanRV32D.Functions.translateAddr addr (AccessType.Read ()) state =
     EStateM.Result.ok (Sail.Ok (physaddr.Physaddr (BitVec.setWidth 34 addr.1), ())) state
   := by
     unfold LeanRV32D.Functions.translateAddr
@@ -384,7 +457,7 @@ namespace Local
       EStateM.bind,
       h_status,
       h_privilege,
-      effective_privilege h_status_val h_access_type,
+      effective_privilege (AccessType.Read ()) privilege state status h_status_val (by trivial),
       translation_mode h_satp,
       h_translation_mode
     ]
@@ -445,76 +518,210 @@ namespace Local
     let z ← x y
     pushGoal z
 
-  example
-    (h_rd: read_xreg (regidx_to_fin rd) state = EStateM.Result.ok rd_val state)
-    (h_alignment: (split_misaligned_pure (virtaddr.Virtaddr (rd_val + offset))) = (1,4))
-    {satp : BitVec 32}
-    (h_status: Sail.readReg Register.mstatus state = EStateM.Result.ok status state)
-    -- (h_tlb: Sail.readReg Register.tlb state = EStateM.Result.ok tlb state)
-    -- (h_tlb_val: ∀ x: Fin 64, tlb[x]! = .none)
-    (h_privilege: Sail.readReg Register.cur_privilege state = EStateM.Result.ok privilege state)
-    (h_status_val:
-      Sail.BitVec.extractLsb status 12 11 = 0#2 ∨
-      Sail.BitVec.extractLsb status 12 11 = 1#2 ∨
-      Sail.BitVec.extractLsb status 12 11 = 3#2
-    )
-    (h_access_type: accessType != AccessType.InstructionFetch ())
-    (h_satp: Sail.readReg Register.satp state = EStateM.Result.ok satp state)
-    (h_translation_mode: translation_mode_pure satp (effective_privilege_pure status privilege) == SATPMode.Bare)
+  lemma pmpReadAddrReg
+    (h_pmp_cfg_n : Sail.readReg Register.pmpcfg_n state = EStateM.Result.ok pmp_cfg_n state)
+    (h_pmp_addr_n : Sail.readReg Register.pmpaddr_n state = EStateM.Result.ok pmp_addr_n state)
   :
-    vmem_read rd offset 4 accessType false false false state =
+    LeanRV32D.Functions.pmpReadAddrReg n state =
+    EStateM.Result.ok pmp_addr_n[n]! state
+  := by
+    unfold LeanRV32D.Functions.pmpReadAddrReg
+    simp [
+      LeanRV32D.Functions.sys_pmp_grain,
+      h_pmp_cfg_n,
+      h_pmp_addr_n
+    ]
+    cases BitVec.ofBool (LeanRV32D.Functions._get_Pmpcfg_ent_A pmp_cfg_n[n]!)[1] with
+      | ofFin x => fin_cases x <;> simp
+
+  /-- We can't prove this directly because the loop in `pmpCheck` doesn't unfold.
+  Adding this is at least consistent, since the left-hand side has no actual value. -/
+  lemma pmp_check_machine_write (reg_val : BitVec 32) (offset : BitVec 32) (width : ℕ) (s) :
+      EStateM.run (
+        LeanRV32D.Functions.pmpCheck (
+          physaddr.Physaddr (
+            LeanRV32D.Functions.zero_extend (
+              Sail.BitVec.addInt (reg_val + offset) 0
+            )
+          )
+        )
+        width
+        (AccessType.Write Data)
+        Privilege.Machine
+      ) s = EStateM.Result.ok none s
+  := by
     sorry
-  := by
-    simp [vmem_read, ext_data_get_addr]
-    unfold liftM monadLift instMonadLiftTOfMonadLift MonadLift.monadLift ExceptT.instMonadLift ExceptT.lift
-    unfold Functor.map ExceptT.mk monadLift instMonadLiftT EStateM.instMonad EStateM.map
-    dsimp
-    unfold bind ExceptT.instMonad ExceptT.bind ExceptT.mk ExceptT.bindCont
-    simp [Sail.SailME.run, ExceptT.run]
-    rewrite [rX_read_xreg_equiv state rd (regidx_to_fin rd) (by simp [regidx_to_fin]), h_rd]
-    simp [
-      ExceptT.pure, ExceptT.mk, check_misaligned, split_misaligned,
-      misaligned_order, LeanRV32D.Functions.zeros
-    ]
-    rewrite [split_misaligned_product, split_misaligned_toNat_product]
-    simp
-    unfold ExceptT.map ExceptT.mk
-    simp [bits_of_virtaddr_of_bits]
-    simp [h_alignment]
-    unfold_projs
-    simp! [Lean.Loop.forIn]
-    get_inaccessible a
 
-    -- generalize _ (_ : Unit → _) _ = x
-
-
-
-
-    -- by_cases h_split: (split_misaligned_pure (virtaddr.Virtaddr (rd_val + offset))) = (1,4)
-    -- . simp [w, w'] at *
-    --   rewrite [h_split]
-    --   simp
-
-    --   done
-    -- . done
-    -- done
-
-
-  example :
-    execute_LOAD imm rs1 rd is_unsigned width state =
-    if width ≤ 4 then
+  /-- We can't prove this directly because the loop in `pmpCheck` doesn't unfold.
+  Adding this is at least consistent, since the left-hand side has no actual value. -/
+  lemma pmp_check_machine_read (reg_val : BitVec 32) (offset : BitVec 32) (width : ℕ) (s) :
+      EStateM.run (
+        LeanRV32D.Functions.pmpCheck (
+          physaddr.Physaddr (
+            LeanRV32D.Functions.zero_extend (
+              Sail.BitVec.addInt (reg_val + offset) 0
+            )
+          )
+        )
+        width
+        (AccessType.Read ())
+        Privilege.Machine
+      ) s = EStateM.Result.ok none s
+    := by
       sorry
-    else
-      EStateM.Result.error (Sail.Error.Assertion "extensions/I/base_insts.sail:287.28-287.29") state
-  := by
-    simp [
-      execute_LOAD,
-      LeanRV32D.Functions.xlen_bytes
-    ]
-    by_cases h_width: width ≤ 4
-    . simp [h_width]
-      done
-    . simp [h_width]
-      done
+
+  -- lemma mem_read
+  --   (rd_val offset: BitVec 32)
+  --   (h_plat_clint_base : Sail.readReg Register.plat_clint_base state = EStateM.Result.ok plat_clint_base state)
+  --   (h_plat_clint_size : Sail.readReg Register.plat_clint_size state = EStateM.Result.ok plat_clint_size state)
+  --   (h_htif_to_host_base : Sail.readReg Register.htif_tohost_base state = EStateM.Result.ok .none state)
+  --   (h_privilege : Sail.readReg Register.cur_privilege state = EStateM.Result.ok privilege state)
+  --   (h_status : Sail.readReg Register.mstatus state = EStateM.Result.ok status state)
+  --   (h_status_val :
+  --     Sail.BitVec.extractLsb status 12 11 = 0#2 ∨
+  --     Sail.BitVec.extractLsb status 12 11 = 1#2 ∨
+  --     Sail.BitVec.extractLsb status 12 11 = 3#2
+  --   )
+  --   (h_machine: effective_privilege_pure status privilege = Privilege.Machine)
+
+  -- :
+  --   LeanRV32D.Functions.mem_read
+  --     (AccessType.Read ())
+  --     (physaddr.Physaddr (BitVec.setWidth 34 (Sail.BitVec.addInt (rd_val + offset) 0)))
+  --     4
+  --     false false false
+  --     state =
+  --   sorry
+  -- := by
+  --   unfold LeanRV32D.Functions.mem_read
+  --   simp [
+  --     h_status,
+  --     h_privilege
+  --   ]
+  --   rewrite [effective_privilege _ _ _ _ h_status_val (by reduce; rfl), h_machine]
+  --   simp [
+  --     LeanRV32D.Functions.mem_read_priv,
+  --     LeanRV32D.Functions.mem_read_priv_meta,
+  --     LeanRV32D.Functions.checked_mem_read,
+  --     LeanRV32D.Functions.phys_access_check,
+  --     LeanRV32D.Functions.sys_pmp_count
+  --   ]
+  --   have h_pmp_check := pmp_check_machine_read rd_val offset 4 state
+  --   simp [
+  --     EStateM.run, LeanRV32D.Functions.zero_extend, Sail.BitVec.zeroExtend
+  --   ] at h_pmp_check
+  --   rewrite [h_pmp_check]
+  --   simp [
+  --     LeanRV32D.Functions.within_mmio_readable,
+  --     LeanRV32D.Functions.get_config_rvfi,
+  --     LeanRV32D.Functions.within_clint,
+  --     h_plat_clint_base,
+  --     h_plat_clint_size,
+  --     LeanRV32D.Functions.within_htif_readable,
+  --     LeanRV32D.Functions.within_htif_writable,
+  --     h_htif_to_host_base,
+  --     Sail.BitVec.addInt
+  --   ]
+  --   rewrite [ite_cond_eq_true]
+  --   . simp [LeanRV32D.Functions.mmio_read]
+  --     done
+  --   . sorry
+
+  --   --17179869184
+  --   --4294967296
+  --   unfold_projs
+  --   simp [Sail.SailME.run, IntRange.forIn']
+  --   unfold IntRange.forIn'.loop
+  --   simp
+  --   rewrite [ite_cond_eq_true]
+  --   . unfold_projs
+  --     simp [Int.lt]
+  --     done
+  --   . unfold_projs
+  --     simp
+  --     reduce
+  --     simp [Int.nonneg_def]
+  --     split_ands <;> [use 0; use 63] <;> simp
+
+  --   done
+
+  -- example
+  --   (h_rd: read_xreg (regidx_to_fin rd) state = EStateM.Result.ok rd_val state)
+  --   (h_alignment: (split_misaligned_pure (virtaddr.Virtaddr (rd_val + offset))) = (1,4))
+  --   {satp : BitVec 32}
+  --   (h_status: Sail.readReg Register.mstatus state = EStateM.Result.ok status state)
+  --   -- (h_tlb: Sail.readReg Register.tlb state = EStateM.Result.ok tlb state)
+  --   -- (h_tlb_val: ∀ x: Fin 64, tlb[x]! = .none)
+  --   (h_privilege: Sail.readReg Register.cur_privilege state = EStateM.Result.ok privilege state)
+  --   (h_status_val:
+  --     Sail.BitVec.extractLsb status 12 11 = 0#2 ∨
+  --     Sail.BitVec.extractLsb status 12 11 = 1#2 ∨
+  --     Sail.BitVec.extractLsb status 12 11 = 3#2
+  --   )
+  --   (h_satp: Sail.readReg Register.satp state = EStateM.Result.ok satp state)
+  --   (h_translation_mode: translation_mode_pure satp (effective_privilege_pure status privilege) == SATPMode.Bare)
+  -- :
+  --   vmem_read rd offset 4 (AccessType.Read ()) false false false state =
+  --   sorry
+  -- := by
+  --   rewrite [vmem_read'_equiv]
+  --   simp [vmem_read', ext_data_get_addr]
+  --   unfold liftM monadLift instMonadLiftTOfMonadLift MonadLift.monadLift ExceptT.instMonadLift ExceptT.lift
+  --   unfold Functor.map ExceptT.mk monadLift instMonadLiftT EStateM.instMonad EStateM.map
+  --   dsimp
+  --   unfold bind ExceptT.instMonad ExceptT.bind ExceptT.mk ExceptT.bindCont
+  --   simp [Sail.SailME.run, ExceptT.run]
+  --   rewrite [rX_read_xreg_equiv state rd (regidx_to_fin rd) (by simp [regidx_to_fin]), h_rd]
+  --   simp [
+  --     ExceptT.pure, ExceptT.mk, check_misaligned, split_misaligned,
+  --     misaligned_order, LeanRV32D.Functions.zeros
+  --   ]
+  --   rewrite [split_misaligned_product, split_misaligned_toNat_product]
+  --   simp
+  --   unfold ExceptT.map ExceptT.mk
+  --   simp [bits_of_virtaddr_of_bits]
+  --   simp [
+  --     h_alignment, untilFuelM, untilFuelM.go
+  --   ]
+  --   rewrite [
+  --     translate_addr h_status h_privilege h_status_val h_satp h_translation_mode,
+  --     h_alignment
+  --   ]
+  --   simp [*]
+  --   unfold_projs
+  --   simp! [Lean.Loop.forIn]
+  --   get_inaccessible a
+
+  --   -- generalize _ (_ : Unit → _) _ = x
+
+
+
+
+  --   -- by_cases h_split: (split_misaligned_pure (virtaddr.Virtaddr (rd_val + offset))) = (1,4)
+  --   -- . simp [w, w'] at *
+  --   --   rewrite [h_split]
+  --   --   simp
+
+  --   --   done
+  --   -- . done
+  --   -- done
+
+
+  -- example :
+  --   execute_LOAD imm rs1 rd is_unsigned width state =
+  --   if width ≤ 4 then
+  --     sorry
+  --   else
+  --     EStateM.Result.error (Sail.Error.Assertion "extensions/I/base_insts.sail:287.28-287.29") state
+  -- := by
+  --   simp [
+  --     execute_LOAD,
+  --     LeanRV32D.Functions.xlen_bytes
+  --   ]
+  --   by_cases h_width: width ≤ 4
+  --   . simp [h_width]
+  --     done
+  --   . simp [h_width]
+  --     done
 
 end Local
