OpenvmFv/Spec/Load/local2.lean
@@ -1,0 +1,324 @@
+import OpenvmFv.Spec.run_hart_active
+import OpenvmFv.Spec.Load.local
+
+
+namespace Local
+  lemma run_vmem_read_of_width_4'
+    (offset : BitVec 32)
+    (data₀ data₁ data₂ data₃ : BitVec 8)
+    (h_aligned : LeanRV32D.Functions.is_aligned_vaddr (virtaddr.Virtaddr (reg_val + offset)) 4 = true)
+    (h_reg_val : LeanRV32D.Functions.rX_bits rs s = EStateM.Result.ok reg_val s)
+    (h_mstatus: Sail.readReg Register.mstatus s = EStateM.Result.ok mstatus s)
+    (h_cur_privilege: Sail.readReg Register.cur_privilege s = EStateM.Result.ok Privilege.Machine s)
+    (h_clint_base: Sail.readReg Register.plat_clint_base s = EStateM.Result.ok 0 s)
+    (h_clint_size: Sail.readReg Register.plat_clint_size s = EStateM.Result.ok 0 s)
+    (h_plat_ram_base: Sail.readReg Register.plat_ram_base s = EStateM.Result.ok 0 s)
+    (h_plat_rom_base: Sail.readReg Register.plat_rom_base s = EStateM.Result.ok 0 s)
+    (h_plat_ram_size: Sail.readReg Register.plat_ram_size s = EStateM.Result.ok (BitVec.ofNat 34 (2^32 - 1)) s)
+    (h_plat_rom_size: Sail.readReg Register.plat_rom_size s = EStateM.Result.ok rom_size s)
+    (h_htif_tohost_base: Sail.readReg Register.htif_tohost_base s = EStateM.Result.ok .none s)
+    (h_mprv_disabled : BitVec.extractLsb 17 17 mstatus = 0#1)
+    (h_does_fit : reg_val.toNat + offset.toNat + 4 < 2^32)
+    (hmem₀ : s.mem[reg_val.toNat + offset.toNat]? = some data₀)
+    (hmem₁ : s.mem[reg_val.toNat + offset.toNat + 1]? = some data₁)
+    (hmem₂ : s.mem[reg_val.toNat + offset.toNat + 2]? = some data₂)
+    (hmem₃ : s.mem[reg_val.toNat + offset.toNat + 3]? = some data₃) :
+    let width := 4
+    let data := data₃ ++ data₂ ++ data₁ ++ data₀
+    (LeanRV32D.Functions.vmem_read
+      rs
+      offset
+      width (AccessType.Read ())
+      false false false
+    ).run s = .ok (.Ok data) s
+  := by
+  rewrite [←vmem_read_equiv, vmem_read'_equiv]
+  have hfetch : (AccessType.Read () != AccessType.InstructionFetch ()) = true := rfl
+  have hsatp_bare : (SATPMode.Bare == SATPMode.Bare) = true := rfl
+  have hmachine : (Privilege.Machine == Privilege.Machine) = true := rfl
+  have hmem₀' : s.mem[(reg_val.toNat + offset.toNat) % 4294967296]? = some data₀ := by
+    rwa [Nat.mod_eq_of_lt]; clear *- h_does_fit; omega
+  have hmem₁' : s.mem[(reg_val.toNat + offset.toNat) % 4294967296 + 1]? = some data₁ := by
+    rwa [Nat.mod_eq_of_lt]; clear *- h_does_fit; omega
+  have hmem₂' : s.mem[(reg_val.toNat + offset.toNat) % 4294967296 + 2]? = some data₂ := by
+    rwa [Nat.mod_eq_of_lt]; clear *- h_does_fit; omega
+  have hmem₃' : s.mem[(reg_val.toNat + offset.toNat) % 4294967296 + 3]? = some data₃ := by
+    rwa [Nat.mod_eq_of_lt]; clear *- h_does_fit; omega
+
+  simp? [
+    Nat.reduceMul, vmem_read',
+    Sail.SailME.run,
+    h_reg_val,
+    h_aligned,
+    LeanRV32D.Functions.ext_data_get_addr,
+    bind_pure_comp, map_pure,
+    liftM_map, bind_map_left,
+    Bool.false_eq_true, ↓reduceIte,
+    LeanRV32D.Functions.plat_enable_misaligned_access,
+    LeanRV32D.Functions.split_misaligned,
+    LeanRV32D.Functions.allowed_misaligned,
+    LeanRV32D.Functions.check_misaligned,
+    CharP.cast_eq_zero, gt_iff_lt, Nat.ofNat_pos,
+    Int.toNat_lt', Nat.cast_ofNat, decide_eq_true_eq,
+    LeanRV32D.Functions.bits_of_virtaddr,
+    Bool.if_false_left,
+    Bool.or_eq_true, Bool.and_eq_true, Bool.not_eq_eq_eq_not,
+    Bool.not_true, decide_eq_false_iff_not, not_lt,
+    Sail.assert, PreSail.assert,
+    beq_iff_eq,
+    LeanRV32D.Functions.misaligned_order,
+    LeanRV32D.Functions.sys_misaligned_order_decreasing,
+    Int.toNat_zero, Int.pred_toNat,
+    Int.toNat_natCast_add_one, Prod.mk.eta, map_bind,
+    Functor.map_map, pure_bind, ExceptT.run_bind, ExceptT.run_monadLift, monadLift_self, ExceptT.run_map,
+    bind_assoc, EStateM.run_bind,
+    EStateM.run, Functor.map, EStateM.map,
+    ExceptT.map, ExceptT.mk, ExceptT.run,
+    liftM, monadLift, MonadLift.monadLift, ExceptT.lift
+  ]
+
+  unfold_projs
+  simp [
+    ExceptT.bind, ExceptT.mk, EStateM.map, h_reg_val,
+    ExceptT.bindCont, ExceptT.pure,
+    h_aligned,
+    untilFuelM,
+    untilFuelM.go
+  ]
+  have h_pmp_check := pmp_check_machine_read reg_val offset 4 s
+  simp [EStateM.run] at h_pmp_check
+  simp [
+    LeanRV32D.Functions.translateAddr,
+    h_mstatus,
+    h_cur_privilege,
+    bind, ExceptT.bind, EStateM.bind, ExceptT.mk,
+    LeanRV32D.Functions.translationMode,
+    LeanRV32D.Functions.effectivePrivilege,
+    hfetch,
+    LeanRV32D.Functions._get_Mstatus_MPRV,
+    Sail.BitVec.extractLsb,
+    h_mprv_disabled,
+    hmachine, hsatp_bare,
+    LeanRV32D.Functions.mem_read,
+    LeanRV32D.Functions.mem_read_priv,
+    LeanRV32D.Functions.mem_read_priv_meta,
+    LeanRV32D.Functions.checked_mem_read,
+    LeanRV32D.Functions.phys_access_check,
+    LeanRV32D.Functions.sys_pmp_count,
+    h_pmp_check,
+    LeanRV32D.Functions.bits_of_virtaddr
+  ]
+
+  simp [
+    LeanRV32D.Functions.within_mmio_readable,
+    LeanRV32D.Functions.get_config_rvfi,
+    LeanRV32D.Functions.within_clint,
+    h_clint_base,
+    h_clint_size,
+    LeanRV32D.Functions.within_htif_readable,
+    LeanRV32D.Functions.within_htif_writable,
+    h_htif_tohost_base,
+    LeanRV32D.Functions.zero_extend,
+    Sail.BitVec.zeroExtend,
+    Sail.BitVec.addInt,
+  ]
+
+  rewrite [ite_cond_eq_false _ _ (by simp; omega)]
+  simp [
+    EStateM.bind,
+    LeanRV32D.Functions.within_phys_mem,
+    h_plat_ram_base,
+    h_plat_rom_base,
+    h_plat_ram_size,
+    h_plat_rom_size
+  ]
+  rewrite [ite_cond_eq_true _ _ (by simp; omega)]
+
+  simp [
+    LeanRV32D.Functions.phys_mem_read,
+    LeanRV32D.Functions.read_kind_of_flags,
+    LeanRV32D.Functions.read_ram,
+    Sail.sail_mem_read, PreSail.sail_mem_read,
+    PreSail.readBytes,
+    PreSail.readByte
+  ]
+  unfold get  instMonadStateOfMonadStateOf getThe MonadStateOf.get EStateM.instMonadStateOf
+  dsimp [EStateM.get]
+
+  have h_mod (n: ℕ) : n % 4294967296 % 17179869184 = n % 4294967296 := by omega
+  rewrite [h_mod]
+
+  simp [
+    hmem₀',
+    hmem₁',
+    hmem₂',
+    hmem₃'
+  ]
+  simp [
+    LeanRV32D.Functions.MemoryOpResult_drop_meta,
+    ExceptT.bindCont,
+    Functor.map, ExceptT.map, ExceptT.mk,
+    Sail.BitVec.updateSubrange,
+    Sail.BitVec.updateSubrange',
+    LeanRV32D.Functions.zeros,
+    Int.sub
+  ]
+
+  example
+    (data₀ data₁ data₂ data₃ : BitVec 8)
+    (h_aligned : LeanRV32D.Functions.is_aligned_vaddr (virtaddr.Virtaddr (reg_val + (BitVec.signExtend 32 imm))) 4 = true)
+    (h_reg_val : LeanRV32D.Functions.rX_bits rs1 s = EStateM.Result.ok reg_val s)
+    (h_mstatus: Sail.readReg Register.mstatus s = EStateM.Result.ok mstatus s)
+    (h_cur_privilege: Sail.readReg Register.cur_privilege s = EStateM.Result.ok Privilege.Machine s)
+    (h_clint_base: Sail.readReg Register.plat_clint_base s = EStateM.Result.ok 0 s)
+    (h_clint_size: Sail.readReg Register.plat_clint_size s = EStateM.Result.ok 0 s)
+    (h_plat_ram_base: Sail.readReg Register.plat_ram_base s = EStateM.Result.ok 0 s)
+    (h_plat_rom_base: Sail.readReg Register.plat_rom_base s = EStateM.Result.ok 0 s)
+    (h_plat_ram_size: Sail.readReg Register.plat_ram_size s = EStateM.Result.ok (BitVec.ofNat 34 (2^32 - 1)) s)
+    (h_plat_rom_size: Sail.readReg Register.plat_rom_size s = EStateM.Result.ok rom_size s)
+    (h_htif_tohost_base: Sail.readReg Register.htif_tohost_base s = EStateM.Result.ok .none s)
+    (h_mprv_disabled : BitVec.extractLsb 17 17 mstatus = 0#1)
+    (h_does_fit : reg_val.toNat + (BitVec.signExtend 32 imm).toNat + 4 < 2^32)
+    (hmem₀ : s.mem[reg_val.toNat + (BitVec.signExtend 32 imm).toNat]? = some data₀)
+    (hmem₁ : s.mem[reg_val.toNat + (BitVec.signExtend 32 imm).toNat + 1]? = some data₁)
+    (hmem₂ : s.mem[reg_val.toNat + (BitVec.signExtend 32 imm).toNat + 2]? = some data₂)
+    (hmem₃ : s.mem[reg_val.toNat + (BitVec.signExtend 32 imm).toNat + 3]? = some data₃)
+  :
+    execute_LOAD imm rs1 rd true 4 s =
+    match LeanRV32D.Functions.wX_bits rd (data₃ ++ data₂ ++ data₁ ++ data₀) s with
+      | EStateM.Result.ok _ s => EStateM.Result.ok (ExecutionResult.Retire_Success ()) s
+      | EStateM.Result.error e s => EStateM.Result.error e s
+  := by
+    have := run_vmem_read_of_width_4'
+      (BitVec.signExtend 32 imm)
+      data₀ data₁ data₂ data₃
+      h_aligned
+      h_reg_val
+      h_mstatus
+      h_cur_privilege
+      h_clint_base
+      h_clint_size
+      h_plat_ram_base
+      h_plat_rom_base
+      h_plat_ram_size
+      h_plat_rom_size
+      h_htif_tohost_base
+      h_mprv_disabled
+      h_does_fit
+      hmem₀ hmem₁ hmem₂ hmem₃
+    simp [EStateM.run] at this
+    simp [
+      execute_LOAD,
+      LeanRV32D.Functions.xlen_bytes,
+      LeanRV32D.Functions.sign_extend,
+      Sail.BitVec.signExtend,
+      LeanRV32D.Functions.Data,
+      this,
+      LeanRV32D.Functions.extend_value, LeanRV32D.Functions.zero_extend, Sail.BitVec.zeroExtend
+    ]
+    aesop
+end Local
+
+
+
+
+
+
+
+
+
+
+
+
+
+
+
+
+
+
+
+
+
+
+#print LeanRV32D.Functions.ext_data_get_addr
+#print LeanRV32D.Functions.vmem_read
+
+noncomputable def vmem_read (rs : regidx) (offset : (BitVec 32)) (width : Nat) (acc : (AccessType Unit)) (aq : Bool) (rl : Bool) (res : Bool) : SailM (Result (BitVec (8 * width)) ExecutionResult) := SailME.run do
+  let vaddr ← (( do
+    match (← (ext_data_get_addr rs offset acc width)) with
+    | .Ext_DataAddr_OK vaddr => (pure vaddr)
+    | .Ext_DataAddr_Error e =>
+      SailME.throw ((Err (Ext_DataAddr_Check_Failure e)) : (Result (BitVec (8 * width)) ExecutionResult))
+    ) : SailME (Result (BitVec (8 * width)) ExecutionResult) virtaddr )
+  if (res : Bool)
+  then
+    (do
+      if ((not (is_aligned_vaddr vaddr width)) : Bool)
+      then
+        SailME.throw ((Err (Memory_Exception (vaddr, (E_Load_Addr_Align ())))) : (Result (BitVec (8 * width)) ExecutionResult))
+      else (pure ()))
+  else
+    (do
+      if ((check_misaligned vaddr width) : Bool)
+      then
+        SailME.throw ((Err (Memory_Exception (vaddr, (E_Load_Addr_Align ())))) : (Result (BitVec (8 * width)) ExecutionResult))
+      else (pure ()))
+  let (n, bytes) ← do (split_misaligned vaddr width)
+  let data := (zeros (n := ((8 *i n) *i bytes)))
+  let (first, last, step) := (misaligned_order n)
+  let i : Nat := first
+  let finished : Bool := false
+  let vaddr := (bits_of_virtaddr vaddr)
+  let (data, finished, i) ← (( do
+    let mut loop_vars := (data, finished, i)
+    repeat
+      let (data, finished, i) := loop_vars
+      loop_vars ← do
+        let offset := i
+        let vaddr := (BitVec.addInt vaddr (offset *i bytes))
+        let data ← (( do
+          match (← (translateAddr (Virtaddr vaddr) acc)) with
+          | .Err (e, _) =>
+            SailME.throw ((Err (Memory_Exception ((Virtaddr vaddr), e))) : (Result (BitVec (8 * width)) ExecutionResult))
+          | .Ok (paddr, _) =>
+            (do
+              match (← (mem_read acc paddr bytes aq rl res)) with
+              | .Err e =>
+                SailME.throw ((Err (Memory_Exception ((Virtaddr vaddr), e))) : (Result (BitVec (8 * width)) ExecutionResult))
+              | .Ok v =>
+                (do
+                  if (res : Bool)
+                  then (load_reservation (bits_of_physaddr paddr))
+                  else (pure ())
+                  (pure (Sail.BitVec.updateSubrange data (((8 *i (offset +i 1)) *i bytes) -i 1)
+                      ((8 *i offset) *i bytes) v)))) ) : SailME
+          (Result (BitVec (8 * width)) ExecutionResult) (BitVec (8 * n * bytes)) )
+        let (finished, i) : (Bool × Nat) :=
+          if ((offset == last) : Bool)
+          then
+            (let finished : Bool := true
+            (finished, i))
+          else
+            (let i : Nat := (offset +i step)
+            (finished, i))
+        (pure (data, finished, i))
+    until (λ (data, finished, i) => finished) loop_vars
+    (pure loop_vars) ) : SailME (Result (BitVec (8 * width)) ExecutionResult)
+    ((BitVec (8 * n * bytes)) × Bool × Nat) )
+  (pure (Ok data))
+
+noncomputable def execute_LOAD (imm : (BitVec 12)) (rs1 : regidx) (rd : regidx) (is_unsigned : Bool) (width: ℕ) : SailM ExecutionResult := do
+    let offset : xlenbits := (LeanRV32D.Functions.sign_extend (m := 32) imm)
+    Sail.assert (width ≤b LeanRV32D.Functions.xlen_bytes) "extensions/I/base_insts.sail:287.28-287.29"
+    match (← (LeanRV32D.Functions.vmem_read rs1 offset width (AccessType.Read LeanRV32D.Functions.Data) false false false)) with
+      | .Ok data =>
+        (do
+          (LeanRV32D.Functions.wX_bits rd (LeanRV32D.Functions.extend_value is_unsigned data))
+          (pure LeanRV32D.Functions.RETIRE_SUCCESS))
+      | .Err e => (pure e)
+
+lemma execute_LOAD_equiv:
+  execute_LOAD =
+  LeanRV32D.Functions.execute_LOAD
+:= by
+  sorry
